sfi/classes.v
@@ -1,0 +1,35 @@
+Require Import eqtype.
+Require Import lib.utils lib.partial_maps lib.ordered common.common.
+
+Section WithClasses.
+
+Generalizable All Variables.
+
+Import PartMaps.
+
+Class abstract_params (t : machine_types) := {
+  memory    :  Type;
+  mem_class :> partial_map memory (word t) (word t);
+  registers :  Type;
+  reg_class :> partial_map registers (reg t) (word t)
+}.
+
+Class params_spec `(ap : abstract_params t) :=
+  { mem_axioms :> PartMaps.axioms (@mem_class t ap)
+  ; reg_axioms :> PartMaps.axioms (@reg_class t ap) }.
+
+Class sfi_syscall_params (t : machine_types) := {
+  (* The registers ISOLATE reads from. *)
+  rIsoA : reg t; rIsoJ : reg t; rIsoS : reg t;
+  
+  (* The location of ISOLATE *)
+  isolate_addr : word t;
+  
+  (* The register the add-to-$SET syscalls read from. *)
+  rAdd : reg t;
+  
+  (* The addresses of the add-to-{J,S} syscalls *)
+  add_to_jump_targets_addr : word t; add_to_shared_memory_addr : word t
+}.
+
+End WithClasses.
