sfi/isolate_sets.v
@@ -1,0 +1,82 @@
+Require Import List Arith Sorted Bool.
+Require Import Coq.Classes.SetoidDec.
+
+Require Import ssreflect ssrfun ssrbool eqtype ssrnat seq.
+
+Require Import lib.utils lib.partial_maps common.common.
+Require Import sfi.ranges sfi.set_utils.
+
+Import DoNotation.
+Import PartMaps.
+
+Generalizable All Variables.
+
+Section WithClasses.
+
+Context  {t            : machine_types}
+         {ops          : machine_ops t}
+         {spec         : machine_ops_spec ops}
+        `{pm           : partial_map Map (word t) V}
+         (to_word      : V -> word t).
+
+Open Scope word_scope.
+
+Definition isolate_get_range (M : Map) (p : word t) : option (list (word t)) :=
+  do! low  <- get M p;
+  do! high <- get M (p + 1);
+  Some (range (to_word low) (to_word high)).
+
+Fixpoint isolate_get_ranges (M : Map)
+                            (p : word t)
+                            (n : nat) : option (list (word t)) :=
+  match n with
+    | O    => Some [::]
+    | S n' => do! here <- isolate_get_range M p;
+              do! rest <- isolate_get_ranges M (p + 2) n';
+              Some (set_union here rest)
+  end.
+
+Definition isolate_create_set (M : Map)
+                              (base : word t) : option (list (word t)) :=
+  do! pairs <- get M base;
+  isolate_get_ranges M (base + 1) (word_to_nat (to_word pairs)).
+
+Local Notation "x ?= y" := (x = Some y) (at level 70, no associativity).
+
+Local Ltac isolate_fn_is_set :=
+  let H := fresh in
+  intros until 0; intros H;
+  let unfix gen f n := first [ gen; induction n; intros; simpl in H;
+                               [solve [inversion H; auto]|]
+                             | unfold f in H; simpl in H ] in
+  match type of H with
+      | ?f ?a ?b ?c ?n ?= ?X => unfix ltac:(gdep c; gdep b; gdep a; gdep X) f n
+      | ?f ?a ?b ?n    ?= ?X => unfix ltac:(gdep b; gdep a; gdep X)         f n
+      | ?f ?a ?n       ?= ?X => unfix ltac:(gdep a; gdep X)                 f n
+      | ?f ?n          ?= ?X => unfix ltac:(gdep X)                         f n
+  end ;
+  repeat match type of H with (do! _ <- ?x; _) ?= _ =>
+    destruct x eqn:?; simpl in H; [|discriminate H]
+  end;
+  inversion H; subst;
+  eauto 4.
+
+Lemma isolate_get_range_is_set : forall M p X,
+  isolate_get_range M p ?= X -> is_set X = true.
+Proof. isolate_fn_is_set. Qed.
+Hint Resolve isolate_get_range_is_set.
+
+Lemma isolate_get_ranges_is_set : forall M p n X,
+  isolate_get_ranges M p n ?= X -> is_set X = true.
+Proof. isolate_fn_is_set. Qed.
+Hint Resolve isolate_get_ranges_is_set.
+
+Lemma isolate_create_set_is_set : forall M base X,
+  isolate_create_set M base ?= X -> is_set X = true.
+Proof. isolate_fn_is_set. Qed.
+
+End WithClasses.
+
+Hint Resolve isolate_get_range_is_set
+             isolate_get_ranges_is_set
+             isolate_create_set_is_set.
