sfi/symbolic.v
@@ -1,0 +1,269 @@
+Require Import List. Import ListNotations.
+
+Require Import ssreflect ssrfun ssrbool eqtype ssrnat seq.
+
+Require Import lib.utils lib.ordered lib.partial_maps common.common.
+Require Import symbolic.symbolic symbolic.rules.
+Require Import sfi.classes sfi.list_utils sfi.set_utils sfi.isolate_sets.
+
+Module Sym.
+
+Section WithClasses.
+
+Import PartMaps.
+
+Context {t            : machine_types}
+        {ops          : machine_ops t}
+        {spec         : machine_ops_spec ops}
+        {sfi_syscalls : sfi_syscall_params t}.
+
+(* I want to use S and I as variables. *)
+Let S := Datatypes.S.
+Let I := Logic.I.
+(* ssreflect exposes `succn' as a synonym for `S' *)
+Local Notation II := Logic.I.
+
+Inductive where_from :=
+| INTERNAL : where_from
+| JUMPED   : where_from.
+
+Inductive stag :=
+| PC     : forall (S : where_from) (c : word t), stag
+| DATA   : forall (c : word t) (I W : list (word t)), stag
+| REG    : stag.
+
+Definition where_from_eq (S1 S2 : where_from) : bool :=
+  match S1, S2 with
+    | INTERNAL , INTERNAL | JUMPED , JUMPED => true
+    | _ , _                                 => false
+  end.
+
+Lemma where_from_eqP : Equality.axiom where_from_eq.
+Proof. by move=> [|] [|] /=; apply: (iffP idP). Qed.
+
+Definition where_from_eqMixin := EqMixin where_from_eqP.
+Canonical where_from_eqType := Eval hnf in EqType where_from where_from_eqMixin.
+
+Definition stag_eq (t1 t2 : stag) : bool :=
+  match t1, t2 with
+    | PC S1 c1      , PC S2 c2      => (S1 == S2) && (c1 == c2)
+    | DATA c1 I1 W1 , DATA c2 I2 W2 => (c1 == c2) && (I1 == I2) && (W1 == W2)
+    | REG           , REG           => true
+    | _             , _             => false
+  end.
+
+Lemma stag_eqP : Equality.axiom stag_eq.
+Proof.
+  by move=> [S1 c1|c1 I1 W1|] [S2 c2|c2 I2 W2|] /=; apply: (iffP idP) => //;
+     do [ do ! move/andP=> []; do ! move=> /eqP->
+        | case; do ! move=> ->; do ! (apply/andP; split) ].
+Qed.
+
+Definition stag_eqMixin := EqMixin stag_eqP.
+Canonical stag_eqType := Eval hnf in EqType stag stag_eqMixin.
+
+Context {memory : Type}
+        {sm : partial_map memory (word t) (atom (word t) stag)}
+        {registers : Type}
+        {sr : partial_map registers (reg t) (atom (word t) stag)}.
+
+Import DoNotation.
+
+Section WithVectors.
+Import Symbolic Coq.Vectors.Vector.VectorNotations.
+
+Definition can_execute (Lpc LI : stag) : option (word t) :=
+  match Lpc , LI with
+    | PC S c , DATA c' I _ =>
+      if      c == c'                       then Some c
+      else if (S == JUMPED) && set_elem c I then Some c'
+      else None
+    | _ , _ => None
+  end.
+
+Definition sfi_rvec (S : where_from) (c : word t) : RVec stag :=
+  mkRVec (PC S c) REG.  
+
+Definition rvec_step (rv : word t -> option (RVec stag))
+                     (Lpc LI : stag)  : option (RVec stag) :=
+  do! c <- can_execute Lpc LI;
+  rv c.
+
+Definition rvec_simple (S : where_from) : stag -> stag -> option (RVec stag) :=
+  rvec_step (fun c => Some (sfi_rvec S c)).
+
+Definition rvec_next : stag -> stag -> option (RVec stag) :=
+  rvec_simple INTERNAL.
+Definition rvec_jump : stag -> stag -> option (RVec stag) :=
+  rvec_simple JUMPED.
+Definition rvec_store (c' : word t) (W : list (word t))
+                      : stag -> stag -> option (RVec stag) :=
+  rvec_step (fun c =>
+    do! guard (c == c') || set_elem c W;
+    Some (sfi_rvec INTERNAL c)).
+
+(* The `REG's in the MVec's fields can also be _s; it's an invariant that
+   registers are always tagged with `REG'. *)
+Definition sfi_handler (mv : MVec stag) : option (RVec stag) :=
+  match mv with
+    | mkMVec NOP       Lpc LI []                      => rvec_next       Lpc LI
+    | mkMVec CONST     Lpc LI [REG]                   => rvec_next       Lpc LI
+    | mkMVec MOV       Lpc LI [REG; REG]              => rvec_next       Lpc LI
+    | mkMVec (BINOP _) Lpc LI [REG; REG; REG]         => rvec_next       Lpc LI
+    | mkMVec LOAD      Lpc LI [REG; DATA _ _ _; REG]  => rvec_next       Lpc LI
+    | mkMVec STORE     Lpc LI [REG; REG; DATA c' _ W] => rvec_store c' W Lpc LI
+    | mkMVec JUMP      Lpc LI [REG]                   => rvec_jump       Lpc LI
+    | mkMVec BNZ       Lpc LI [REG]                   => rvec_next       Lpc LI
+    | mkMVec JAL       Lpc LI [REG; REG]              => rvec_jump       Lpc LI
+    | mkMVec _         _   _  _                       => None
+  end.
+
+End WithVectors.
+
+Record sfi_internal := Internal { next_id : word t
+                                ; set_ids : list (list (word t) * word t) }.
+
+Instance sym_sfi : Symbolic.symbolic_params := {
+  tag := stag_eqType;
+  
+  handler := sfi_handler;
+  
+  internal_state := sfi_internal;
+  
+  memory := memory;
+  sm     := sm;
+  
+  registers := registers;
+  sr        := sr
+}.
+
+Notation "'do!' ( X , Y ) <- A ; B" :=
+  (bind (fun XY => let '(X,Y) := XY in B) A)
+  (at level 200, X ident, Y ident, A at level 100, B at level 200).
+
+Notation "'do!' X @ L <- A ; B" :=
+  (bind (fun XL => let '(X @ L) := XL in B) A)
+  (at level 200, X ident, L ident, A at level 100, B at level 200).
+
+Notation "'do!' X @ 'REG' <- A ; B" :=
+  (bind (fun XREG => match XREG with | X @ REG => B | _ => None end) A)
+  (at level 200, X ident, A at level 100, B at level 200).
+
+Notation "'do!' X @ 'DATA' c I W <- A ; B" :=
+  (bind (fun XcIW => match XcIW with | X @ (DATA c I W) => B | _ => None end) A)
+  (at level 200, X ident, c ident, I ident, W ident,
+   A at level 100, B at level 200).
+
+Notation "'do!' 'REG' <- A ; B" :=
+  (bind (fun maybeREG => match maybeREG with | REG => B | _ => None end) A)
+  (at level 200, A at level 100, B at level 200).
+
+Notation "'do!' 'DATA' c I W <- A ; B" :=
+  (bind (fun cIW => match cIW with | DATA c I W => B | _ => None end) A)
+  (at level 200, c ident, I ident, W ident, A at level 100, B at level 200).
+
+Notation "'do!' 'REG' <-! A ; B" :=
+  (match A with | REG => B | _ => None end)
+  (at level 200, A at level 100, B at level 200).
+
+Notation "'do!' 'DATA' c I W <-! A ; B" :=
+  (match A with | DATA c I W => B | _ => None end)
+  (at level 200, c ident, I ident, W ident, A at level 100, B at level 200).
+
+Definition fresh (si : sfi_internal) : option (word t * sfi_internal) :=
+  let 'Internal next ids := si in
+  if next == max_word
+  then None
+  else Some (next, Internal (next+1)%w ids).
+
+Definition register_set (X : list (word t))
+                        (si : sfi_internal) : option sfi_internal :=
+  let 'Internal next ids := si in
+  match assoc_list_lookup ids (eq_op X) with
+    | Some _ => Some si
+    | None   => do! (id,si') <- fresh si;
+                Some (Internal (next_id si') ((X,id) :: set_ids si'))
+  end.  
+
+Fixpoint retag_set (ok : word t -> list (word t) -> list (word t) -> bool)
+                   (retag : word t -> list (word t) -> list (word t) -> stag)
+                   (ps : list (word t))
+                   (M : memory) (si : sfi_internal)
+                   : option (memory * sfi_internal) :=
+  match ps with
+    | []       => Some (M,si)
+    | p :: ps' => do! x @ L          <-  get M p;
+                  do! x @ DATA c I W <-  get M p;
+                  do! guard (ok c I W);
+                  do! DATA _ I' W'   <-! retag c I W;
+                  do! si'            <-  register_set I' si;
+                  do! si''           <-  register_set W' si;
+                  do! M'             <-  upd M p (x @ L);
+                  retag_set ok retag ps' M' si''
+  end.
+
+Definition isolate (s : Symbolic.state t) : option (Symbolic.state t) :=
+  match s with
+    | Symbolic.State M R (pc @ (PC _ c)) si =>
+      do! (c',si') <- fresh si;
+      
+      do! pA @ _ <- get R rIsoA;
+      do! pJ @ _ <- get R rIsoJ;
+      do! pS @ _ <- get R rIsoS;
+      
+      do! A'       <- isolate_create_set (@val _ _) M pA;
+      do! guard nonempty A';
+      do! (MA,siA) <- retag_set (fun c'' _ _ => c == c'')
+                                (fun _   I W => DATA c' I W)
+                                A' M si';
+      
+      do! J'       <- isolate_create_set (@val _ _) M pJ;
+      do! (MJ,siJ) <- retag_set (fun c'' I _ => (c == c'') || set_elem c I)
+                                (fun c'' I W => DATA c'' (insert_unique c' I) W)
+                                J' MA siA;
+      
+      do! S'       <- isolate_create_set (@val _ _) M pS;
+      do! (MS,siS) <- retag_set (fun c'' _ W => (c == c'') || set_elem c W)
+                                (fun c'' I W => DATA c'' I (insert_unique c' W))
+                                J' MJ siJ;
+
+      Some (Symbolic.State MS R ((pc + 1)%w @ (PC INTERNAL c)) siS)
+    | _ => None
+  end.
+
+Definition add_to_jump_targets (s : Symbolic.state t)
+                               : option (Symbolic.state t) :=
+  match s with
+    | Symbolic.State M R (pc @ (PC _ c)) si =>
+      do! p @ _           <- get R rAdd;
+      do! x @ DATA c' I W <- get M p;
+      let I'              := insert_unique c I in
+      do! si'             <- register_set I' si;
+      do! M'              <- upd M p (x @ (DATA c' I' W));
+      Some (Symbolic.State M' R ((pc + 1)%w @ (PC INTERNAL c)) si')
+    | _ => None
+  end.
+
+Definition add_to_shared_memory (s : Symbolic.state t)
+                               : option (Symbolic.state t) :=
+  match s with
+    | Symbolic.State M R (pc @ (PC _ c)) si =>
+      do! p @ _           <- get R rAdd;
+      do! x @ DATA c' I W <- get M p;
+      let W'              := insert_unique c W in
+      do! si'             <- register_set W' si;
+      do! M'              <- upd M p (x @ (DATA c' I W'));
+      Some (Symbolic.State M' R ((pc + 1)%w @ (PC INTERNAL c)) si')
+    | _ => None
+  end.
+
+Definition syscalls : list (Symbolic.syscall t) :=
+  [Symbolic.Syscall isolate_addr              isolate;
+   Symbolic.Syscall add_to_jump_targets_addr  add_to_jump_targets;
+   Symbolic.Syscall add_to_shared_memory_addr add_to_shared_memory].
+
+Definition step := Symbolic.step syscalls.
+
+End WithClasses.
+
+End Sym.
